LeanCats.lean
@@ -11,10 +11,8 @@ import LeanCats.Theorems
 import LeanCats.TsoWeakerThanSc
 import LeanCats.mipsWeakerThanTSO
 import LeanCats.ModelReader
-import LeanCats.Litmus
 import LeanCats.LitmusParser
 import LeanCats.LitmusGraph
 import LeanCats.LitmusGraphBridge
 import LeanCats.LitmusReader
 import LeanCats.Linux.CoRR_poonceonce_Once
-import LeanCats.Linux.X86_SB_rfi_pos
