LeanCats/Linux/IRIW.lean
@@ -1,0 +1,118 @@
+import LeanCats.Basic
+import LeanCats.Data
+import LeanCats.Macro
+import LeanCats.Theorems
+
+open Data
+
+namespace LinuxLitmus
+
+instance instWellformedPo (evts : Data.Events) : wellformed.po evts.po := by
+  intro x y z hxy hyz
+  rcases hxy with ⟨hx, hy, hxyTid, hxyLt⟩
+  rcases hyz with ⟨_, hz, hyzTid, hyzLt⟩
+  exact ⟨hx, hz, Eq.trans hxyTid hyzTid, Nat.lt_trans hxyLt hyzLt⟩
+
+instance instWellformedRmwEmpty (evts : Data.Events) : wellformed.rmw evts (∅ : SetRel Event Event) := by
+  intro e h
+  contradiction
+
+abbrev x := 0
+abbrev y := 1
+
+@[simp] abbrev initOpX : Data.Effect :=
+  Data.Effect.mk Data.Op.write x (some 0) true false
+@[simp] abbrev initOpY : Data.Effect :=
+  Data.Effect.mk Data.Op.write y (some 0) true false
+@[simp] abbrev wOpX1 : Data.Effect :=
+  Data.Effect.mk Data.Op.write x (some 1) false false
+@[simp] abbrev wOpY1 : Data.Effect :=
+  Data.Effect.mk Data.Op.write y (some 1) false false
+@[simp] abbrev rOpX1 : Data.Effect :=
+  Data.Effect.mk Data.Op.read x (some 1) false false
+@[simp] abbrev rOpY1 : Data.Effect :=
+  Data.Effect.mk Data.Op.read y (some 1) false false
+@[simp] abbrev rOpX0 : Data.Effect :=
+  Data.Effect.mk Data.Op.read x (some 0) false false
+@[simp] abbrev rOpY0 : Data.Effect :=
+  Data.Effect.mk Data.Op.read y (some 0) false false
+
+@[simp] abbrev initWx : Data.Event :=
+  Data.Event.mk 100 10 initOpX ⟨lkmm.Accesses, lkmm.Accesses.ONCE'⟩
+@[simp] abbrev initWy : Data.Event :=
+  Data.Event.mk 101 10 initOpY ⟨lkmm.Accesses, lkmm.Accesses.ONCE'⟩
+
+@[simp] abbrev p0wX1 : Data.Event :=
+  Data.Event.mk 1 0 wOpX1 ⟨lkmm.Accesses, lkmm.Accesses.ONCE'⟩
+
+@[simp] abbrev p1rX1 : Data.Event :=
+  Data.Event.mk 2 1 rOpX1 ⟨lkmm.Accesses, lkmm.Accesses.ONCE'⟩
+@[simp] abbrev p1rY0 : Data.Event :=
+  Data.Event.mk 3 1 rOpY0 ⟨lkmm.Accesses, lkmm.Accesses.ONCE'⟩
+
+@[simp] abbrev p2wY1 : Data.Event :=
+  Data.Event.mk 4 2 wOpY1 ⟨lkmm.Accesses, lkmm.Accesses.ONCE'⟩
+
+@[simp] abbrev p3rY1 : Data.Event :=
+  Data.Event.mk 5 3 rOpY1 ⟨lkmm.Accesses, lkmm.Accesses.ONCE'⟩
+@[simp] abbrev p3rX0 : Data.Event :=
+  Data.Event.mk 6 3 rOpX0 ⟨lkmm.Accesses, lkmm.Accesses.ONCE'⟩
+
+@[simp] abbrev iriw_evts : Data.Events :=
+  Data.Events.mk
+    {initWx, initWy}
+    {p1rX1, p1rY0, p3rY1, p3rX0}
+    {initWx, initWy, p0wX1, p2wY1}
+    {}
+    {}
+    {}
+
+@[simp] def iriw_co : SetRel Event Event :=
+  {(initWx, p0wX1), (initWy, p2wY1)}
+
+instance : wellformed.co iriw_evts iriw_co where
+  irrefl := by aesop
+  trans := by aesop
+  preco := {
+    wellTyped := by aesop
+    total := by candidateExecution_wf
+  }
+
+@[simp] def iriw_rf : SetRel Event Event :=
+  {(p0wX1, p1rX1), (initWy, p1rY0), (p2wY1, p3rY1), (initWx, p3rX0)}
+
+@[simp] def iriw_rfInst : wellformed.rf iriw_evts iriw_rf :=
+  Data.wellformed.rf.mk
+    (by
+      candidateExecution_wf
+    )
+    (by
+      candidateExecution_wf
+    )
+
+@[simp] def iriw_mb : SetRel Event Event :=
+  {(p1rX1, p1rY0), (p3rY1, p3rX0)}
+
+@[simp] def iriw_test : CandidateExecution iriw_evts :=
+  {
+    evts := iriw_evts
+    po' := iriw_evts.po
+    prePo := instWellformedPo iriw_evts
+    rf' := iriw_rf
+    rfInst := iriw_rfInst
+    co' := iriw_co
+    rmw' := ∅
+    preRMW := instWellformedRmwEmpty iriw_evts
+    mb' := iriw_mb
+    uniqueId := uniqueId_by_id iriw_evts
+    syncInF := by
+      intro e h
+      contradiction
+    rfiPo := by
+      candidateExecution_wf
+  }
+
+theorem iriw_disallowed : ¬ lkmm.propagation iriw_evts iriw_test := by
+  native_decide
+
+end LinuxLitmus
